
\documentclass[12pt, reqno]{amsart}
\usepackage{geometry} % see geometry.pdf on how to lay out the page. There's lots.
\geometry{a4paper} % or letter or a5paper or ... etc
% \geometry{landscape} % rotated page geometry

% See the ``Article customise'' template for come common customisations

\usepackage{braket}
\usepackage{amsmath}

\title{cQED Problems}
\author{Matthew Beck}
\date{March 27, 2017} % delete this line to display the current date

%%% BEGIN DOCUMENT
\begin{document}

\maketitle
%\tableofcontents

\section{Prove $e^{i\delta} \ket{n} = \ket{n+1}$}
%\subsection{}

Beginning with the commutation relation $[\hat{\delta},\hat{n}] = i$ and $\hat{n} = \frac{1}{i}\frac{\partial}{\partial \delta}$

\begin{align}
[e^{i\hat{\delta}},\hat{n}] \ket{\psi} &= (e^{i\hat{\delta}}\hat{n} - \hat{n}e^{i\hat{\delta}})\ket{\psi} \\
&= e^{i\hat{\delta}} \frac{1}{i}\frac{\partial \ket{\psi}}{\partial \delta} - e^{i\hat{\delta}} \frac{1}{i}\frac{\partial \ket{\psi}}{\partial \delta} - e^{i \hat{\delta}} \ket{\psi} \\
&=  - e^{i \hat{\delta}} \ket{\psi} \label{eqn3}
\end{align}

We can now use the results of (\ref{eqn3}) we can find $\hat{n}e^{i\hat{\delta}}\ket{n}$

\begin{align}
\hat{n}e^{i\hat{\delta}}\ket{n} &= \hat{n}e^{i\hat{\delta}}\ket{n} -e^{i\hat{\delta}} \hat{n}\ket{n} + e^{i\hat{\delta}} \hat{n}\ket{n} \\
&= [\hat{n}, e^{i\hat{\delta}}] + e^{i\hat{\delta}} \hat{n}\ket{n} \\
&= e^{i \hat{\delta}} \ket{\psi}  + e^{i\hat{\delta}} \hat{n}\ket{n} \\
&= e^{i \hat{\delta}} \ket{\psi}  + e^{i\hat{\delta}} n\ket{n} \\
&= (n+1) e^{i\hat{\delta}}\ket{n} \label{eqn8}
\end{align}

We can equate (\ref{eqn8}) as

\begin{align}
(n+1) e^{i\hat{\delta}}\ket{n} \equiv \hat{n} \ket{n+1}
\end{align}

which inherently defines

\begin{align}
 e^{i\hat{\delta}}\ket{n} = \ket{n+1}
\end{align}


\end{document}
